map_types

lambda2Gmu/TestVector.v
@@ -1,4 +1,5 @@
 Require Import TestCommon.
+Require Import Equations.
 
 (*
 
@@ -31,9 +32,6 @@ we can create a vector containing two units:
   uvec = (cons () (cons () empty)) // I skip the type args here, they are elaborated in the proof
   uvec : Vector Unit (Succ (Succ Zero))
 
->> ^ this is implemented
->> the things below are not (yet) because pattern matching is not yet done and they require it
-
 we can create a map function that guarantees that it preserves length:
   map : forall a b n, (a -> b) -> Vector a n -> Vector b n
 
@@ -59,6 +57,8 @@ Axiom Vector : var.
 Open Scope L2GMu.
 Axiom all_distinct :
   (Zero <> Succ) /\ (Succ <> Vector) /\ (Zero <> Vector).
+
+(* De Bruijn indices for arguments are in 'reverse' order, that is the last arg on the list is treated as 'closest' and referred to as ##0 *)
 Definition VectorDef := (* Vector a len *)
   enum 2 {{
          (* empty : () -> Vector a Zero *)
@@ -92,8 +92,11 @@ Lemma oksigma : okGadt sigma.
       repeat rewrite union_empty_r; auto.
 Qed.
 
-Definition nil A := new (Vector, 0) [| A |] (trm_unit).
-Definition cons A N h t := new (Vector, 1) [|A, N|]  (trm_tuple h t).
+Definition Nil := (Vector, 0).
+Definition Cons := (Vector, 1).
+
+Definition nil A := new Nil [| A |] (trm_unit).
+Definition cons A N h t := new Cons [|A, N|]  (trm_tuple h t).
 
 Lemma nil_type : {sigma, emptyΔ, empty} ⊢(Treg) (Λ => nil (##0)) ∈ typ_all (γ(##0, γ() Zero) Vector).
   cbv.
@@ -145,4 +148,225 @@ Lemma uvec2_type : {sigma, emptyΔ, empty} ⊢(Treg) uvec2 ∈ γ(typ_unit, two)
   lets: oksigma.
   lets [? [? ?]]: all_distinct.
   autotyper1.
+Qed.
+
+(*
+  map : forall a b n, (a -> b) -> Vector a n -> Vector b n
+ *)
+Definition map :=
+  fixs ∀ ∀ ∀ ((##2 ==> ##1) ==> γ(##2, ##0) Vector ==> γ(##1, ##0) Vector) =>
+  Λ => Λ => Λ =>
+  λ (##2 ==> ##1) =>
+  λ γ(##2, ##0) Vector =>
+  case #0 as Vector of {
+                      bind 1 in new Nil [| ##2 |] ( <.> ) |
+                      bind 2 in new Cons [| ##3, ##0 |] (
+                                      trm_tuple
+                                        (#2 <| fst(#0))
+                                        (#3 <|| ##4 <|| ##3 <|| ##0 <| #2 <| snd(#0))
+                                    )
+                    }.
+
+             (* TODO merge with autotyper1 *)
+Ltac autotyper0 :=
+  repeat progress (
+           cbn;
+           match goal with
+           | [ H: False |- _ ] => false*
+           | [ |- ok ?A ] => econstructor
+           | [ |- okt ?A ?B ?C ] => econstructor
+           | [ |- binds ?A ?B ?C ] => solve_bind
+           | [ |- ?A \notin ?B ] => simpl_dom; notin_solve; try (apply notin_singleton)
+           | [ |- forall x, x \notin ?L -> ?P ] =>
+             let free := gather_vars in
+             let x' := fresh "x" in
+             let xiL := fresh "xiL" in
+             intros x' xiL; intros;
+             try instantiate (1 := free) in xiL
+           | [ |- okGadt empty ] => econstructor
+           | [ |- wft ?A ?B ?C ] => econstructor
+           | [ |- value ?A ] => econstructor
+           | [ |- term ?A ] => econstructor
+           | [ |- type ?A ] => econstructor
+           | [ H: binds ?A ?B ?C |- _ ] => binds_inv
+           | [ |- ?A /\ ?B ] => split
+           | [ H: {| Tarity := ?A; Tconstructors := ?B |} = ?C |- _ ] =>
+             inversions H
+           | [ H: ?A \/ ?B |- _ ] => destruct H
+           | [ |- is_var_defined (?A |,| ?B) ?c ] => apply is_var_defined_split
+           | _ => intros; auto
+           end;
+           cbn; subst).
+
+Lemma neq_from_notin : forall (A : Type) (x y : A), x \notin \{ y } -> x <> y.
+  intros.
+  intro HF.
+  subst.
+  apply* notin_same.
+Qed.
+
+Ltac autotyper2 :=
+  repeat progress (
+           cbn;
+           match goal with
+           | [ H: False |- _ ] => false*
+           | [ |- ok ?A ] => econstructor
+           | [ |- okt ?A ?B ?C ] => econstructor
+           | [ |- binds ?A ?B ?C ] => solve_bind
+           | [ |- typing ?TT ?A ?B ?C (trm_unit) ?E ] => eapply typing_unit
+           | [ |- typing ?TT ?A ?B ?C (trm_fvar ?X) ?E ] => eapply typing_var
+           | [ |- typing ?TT ?A ?B ?C (trm_constructor ?Ts ?N ?e) ?E ] => eapply typing_cons
+           | [ |- typing ?TT ?A ?B ?C (trm_abs ?T ?e) ?E ] => eapply typing_abs
+           | [ |- typing ?TT ?A ?B ?C (trm_tabs ?e) ?E ] => eapply typing_tabs
+           | [ |- typing ?TT ?A ?B ?C (trm_app ?e1 ?e2) ?E ] => eapply typing_app
+           | [ |- typing ?TT ?A ?B ?C (trm_tapp ?e1 ?T) ?E ] => eapply typing_tapp
+           | [ |- typing ?TT ?A ?B ?C (trm_tuple ?e1 ?e2) ?E ] => eapply typing_tuple
+           | [ |- typing ?TT ?A ?B ?C (trm_fst ?e1) ?E ] => eapply typing_fst
+           | [ |- typing ?TT ?A ?B ?C (trm_snd ?e1) ?E ] => eapply typing_snd
+           | [ |- typing ?TT ?A ?B ?C (trm_fix ?T ?e) ?E ] => eapply typing_fix
+           | [ |- typing ?TT ?A ?B ?C (trm_let ?e1 ?e2) ?E ] => eapply typing_let
+           | [ |- typing ?TT ?A ?B ?C (trm_matchgadt ?e1 ?N ?ms) ?E ] => eapply typing_case
+           | [ |- ?A \notin ?B ] => simpl_dom; notin_solve; try (apply notin_singleton)
+           | [ |- forall x, x \notin ?L -> ?P ] =>
+             let free := gather_vars in
+             let x' := fresh "x" in
+             let xiL := fresh "xiL" in
+             intros x' xiL; intros;
+             try instantiate (1 := free) in xiL
+           | [ |- okGadt empty ] => econstructor
+           | [ |- wft ?A ?B ?C ] => econstructor
+           | [ |- value ?A ] => econstructor
+           | [ |- term ?A ] => econstructor
+           | [ |- type ?A ] => econstructor
+           | [ H: binds ?A ?B ?C |- _ ] => binds_inv
+           | [ |- ?A /\ ?B ] => split
+           | [ H: {| Tarity := ?A; Tconstructors := ?B |} = ?C |- _ ] =>
+             inversions H
+           | [ H: ?A \/ ?B |- _ ] => destruct H
+           | [ H: ?C = (?A, ?B) |- _ ] => inversions H
+           | [ H: (?A, ?B) = ?C |- _ ] => inversions H
+           | [ |- is_var_defined (?A |,| ?B) ?c ] => apply is_var_defined_split
+           | _ => intros; auto
+           end;
+           cbn; subst).
+
+Ltac autotyper3 :=
+  autotyper2; cbn in *;
+  destruct_const_len_list; cbn; autotyper2.
+
+Ltac autotyper4 :=
+  autotyper3;
+  try solve [left~ | repeat right~].
+
+Lemma Forall2_eq : forall A B (f : A -> B) Ts Us,
+    List.length Ts = List.length Us ->
+    (forall T U, List.In (T, U) (zip Ts Us) -> f T = f U) ->
+    List.map f Ts =
+    List.map f Us.
+  induction Ts as [ | T Ts]; destruct Us as [ | U Us]; intros Len F; cbn in *; inversion Len.
+  - auto.
+  - f_equal; auto.
+Qed.
+
+Lemma eq_typ_gadt : forall Σ Δ Ts Us N,
+    List.Forall2 (fun T U => entails_semantic Σ Δ (T ≡ U)) Ts Us ->
+    entails_semantic Σ Δ (typ_gadt Ts N ≡ typ_gadt Us N).
+  introv FF.
+  cbn in *.
+  apply F2_iff_In_zip in FF.
+  destruct FF.
+  intros O M.
+  repeat rewrite subst_tt_prime_reduce_typ_gadt.
+  f_equal.
+  apply~ Forall2_eq.
+Qed.
+
+Ltac ininv2 :=
+  match goal with
+  | H: List.In _ _ |- _ =>
+    inversions H
+  | [ H: ?C = (?A, ?B) |- _ ] => inversions H
+  | [ H: (?A, ?B) = ?C |- _ ] => inversions H
+  end.
+
+Lemma map_types : {sigma, emptyΔ, empty} ⊢(Treg) map ∈ ∀ ∀ ∀ ((##2 ==> ##1) ==> γ(##2, ##0) Vector ==> γ(##1, ##0) Vector).
+  cbv.
+  lets: oksigma.
+  lets [? [? ?]]: all_distinct.
+autotyper3;
+    rename x0 into map;
+    rename x into A;
+    rename x1 into B;
+    rename x2 into N;
+    rename x3 into f;
+    rename x4 into vec;
+    rename x5 into elem.
+  - instantiate (1:=\{x} \u \{ x0 } \u \{ x1 } \u \{ x2 } \u \{ x3 } \u \{ x4 }) in H7.
+    rename v into C.
+    forwards~ : H6 C.
+    apply typing_eq with (γ(typ_fvar B, γ() Zero) Vector) Treg.
+    + autotyper4.
+    + apply eq_typ_gadt.
+      apply F2_iff_In_zip.
+      split~.
+      intros.
+      repeat ininv2.
+      * apply teq_symmetry.
+        apply teq_axiom. listin.
+      * apply teq_reflexivity.
+    + autotyper4.
+  - rename v0 into A'.
+    rename v into N'.
+    forwards~ : H6 A'.
+    forwards~ : H6 N'.
+    apply typing_eq with (γ(typ_fvar B, γ(typ_fvar N') Succ) Vector) Treg.
+    + eapply typing_cons; autotyper0.
+      * eapply typing_tuple; autotyper0.
+        -- econstructor.
+           ++ instantiate (1:=A).
+              apply typing_eq with A' Treg.
+              ** autotyper4.
+              ** apply teq_symmetry. apply teq_axiom. listin.
+              ** autotyper4.
+           ++ autotyper4.
+        -- econstructor; autotyper0.
+           instantiate (1:= γ(typ_fvar A, typ_fvar N') Vector).
+           ++ apply typing_eq with (γ(typ_fvar A', typ_fvar N') Vector) Treg.
+              ** autotyper4.
+              ** apply eq_typ_gadt.
+                 apply F2_iff_In_zip.
+                 split~.
+                 intros.
+                 repeat ininv2.
+                 --- apply teq_reflexivity.
+                 --- apply teq_symmetry.
+                     apply teq_axiom. listin.
+              ** autotyper4.
+           ++ autotyper4.
+      * autotyper4.
+    + apply eq_typ_gadt.
+      apply F2_iff_In_zip.
+      split~.
+      intros.
+      repeat ininv2.
+      * apply teq_symmetry.
+        apply teq_axiom. listin.
+      * apply teq_reflexivity.
+    + autotyper4.
+      Unshelve.
+      fs.
+      fs.
+      fs.
+      fs.
+      fs.
+      fs.
+      fs.
+      fs.
+      fs.
+      fs.
+      fs.
+      fs.
+      fs.
+      fs.
+      fs.
 Qed.
